progress on leader_election

chapter04/solutions/leader_election.dfy
@@ -1,28 +1,111 @@
-// TODO Manos suggests using modulo for positions instead of links
-datatype NodeConstants = NodeConstants(neighbor: nat)
-datatype Node = Node(highest_heard: nat)
+// Each node's identifier (address)
+datatype Constants = Constants(ids: seq<nat>)
 
-datatype Constants = Constants(nodes: seq<Node>)
-datatype Variables = Variables(nodes: seq<Node>)
+// The highest other identifier this node has heard about.
+datatype Variables = Variables(highest_heard: seq<nat>)
 
-predicate IsLeader(k: Constants, s: Variables, i: nat)
-{
-  s.nodes[i].highest_heard == i
+predicate ValidIdx(k: Constants, i: nat) {
+  0<=i<|k.ids|
 }
 
-predicate Safety(k: Constants, s: Variables)
-{
-  forall i, j | IsLeader(k, s, i) && IsLeader(k, s, j) :: i == j
+predicate WF(k: Constants, s: Variables) {
+  && 0 < |k.ids|
+  && |s.highest_heard| == |k.ids|
 }
 
-predicate Receive(k: Constants, s: Variables, s': Variables, src: nat, dst: nat)
+predicate Init(k: Constants, s: Variables)
 {
-  && k.nodes
-  && var neighbor_highest := 
-  && s' == s.[dst := Node(neighbor_highest)]
+  && WF(k, s)
+    // Everyone begins having heard about nobody, not even themselves.
+  && (forall i | ValidIdx(k, i) :: s.highest_heard[i] == 0)
+    // No two nodes have the same identifier.
+  && (forall i, j | ValidIdx(k, i) && ValidIdx(k, j) && k.ids[i]==k.ids[j]
+    :: i == j)
+}
+
+function max(a: nat, b: nat) : nat {
+  if a > b then a else b
+}
+
+predicate Transmission(k: Constants, s: Variables, s': Variables, src: nat)
+{
+  && WF(k, s)
+  && WF(k, s')
+  && 0 <= src < |k.ids|
+
+  // Neighbor address in ring.
+  // TODO let's try it with modulo, too.
+  // var dst := if src + 1 < |s.nodes| then src + 1 else 0;
+  && var dst := (src + 1) % |k.ids|;
+
+  // src sends its highest_heard value
+  && var message := s.highest_heard[src];
+
+  // dst updates its highest_heard with the max of the message and its own id
+  && var dst_new_highest := max(message, k.ids[dst]);
+
+  && s' == s.(highest_heard := s.highest_heard[dst := dst_new_highest])
+}
+
+datatype Step = TransmissionStep(src: nat)
+
+predicate NextStep(k: Constants, s: Variables, s': Variables, step: Step)
+{
+  match step {
+    case TransmissionStep(src) => Transmission(k, s, s', src)
+  }
 }
 
 predicate Next(k: Constants, s: Variables, s': Variables)
 {
-  && 
+  exists step :: NextStep(k, s, s', step)
 }
+
+predicate IsLeader(k: Constants, s: Variables, i: nat)
+  requires WF(k, s)
+{
+  && ValidIdx(k, i)
+  && s.highest_heard[i] == k.ids[i]
+}
+
+// TODO note that the elected leader isn't stable, which isn't ideal.
+predicate Safety(k: Constants, s: Variables)
+  requires WF(k, s)
+{
+  forall i, j | IsLeader(k, s, i) && IsLeader(k, s, j) :: i == j
+}
+
+predicate IsMaxId(k: Constants, id: nat)
+{
+  forall j | ValidIdx(k, j) :: k.ids[j] <= id
+}
+
+predicate Inv(k: Constants, s: Variables)
+{
+  && WF(k, s)
+  && Safety(k, s)
+  && (forall i | ValidIdx(k, i) && !IsMaxId(k, i) :: !IsLeader(k, s, i))
+}
+
+lemma InitImpliesInv(k: Constants, s: Variables)
+  requires Init(k, s)
+  ensures Inv(k, s)
+{
+  forall i | ValidIdx(k, i) && !IsMaxId(k, i) && IsLeader(k, s, i)
+    ensures false
+  {
+    if k.ids[i]!=0 {
+      assert false;
+    } else {
+      assert false;
+    }
+  }
+}
+
+lemma NextPreservesInv(k: Constants, s: Variables, s': Variables)
+  requires Inv(k, s)
+  requires Next(k, s, s')
+  ensures Inv(k, s')
+{
+}
+
